

```

In[*]:= M3 = {{-(ℓ c γ) - c Subscript[r, x], c Subscript[r, x]},
               {β (1 - ℓ c γ - c Subscript[r, x]), -β + β c Subscript[r, x]}} // MatrixForm
               [下角标] [下角标] [下角标] [矩阵格式]

{val, vec} = Eigensystem[M3];
               [特征系统]

val[[2]] (* The eigenvalue of M1 *)
{1, vecs[[2]] [[2]] / vecs[[2]] [[1]]} (* Corresponding eigenvector *)

Out[*]//MatrixForm=

$$\begin{pmatrix} -c \ell \gamma - c r_x & c r_x \\ \beta (1 - c \ell \gamma - c r_x) & -\beta + c \beta r_x \end{pmatrix}$$


[Set: 列表 {val, vec} 和 Eigensystem[ $\begin{pmatrix} -c \ell \gamma - c r_x & c r_x \\ \beta (1 - c \ell \gamma - c \text{Subscript}[\ll 2 \gg]) & -\beta + c \beta r_x \end{pmatrix}$ ] 形状不同.]

Out[*]=

$$\frac{1}{2} \left( -\beta - c \ell \gamma - c r_x + c \beta r_x + \sqrt{-4 c \ell \beta \gamma + (\beta + c \ell \gamma + c r_x - c \beta r_x)^2} \right)$$


Out[*]=

$$\left\{ 1, -\frac{2 b (1 + c \ell) \alpha}{-c \ell - b^2 c \alpha - \alpha r_y - \sqrt{c^2 \ell^2 - 4 b^2 c \alpha - 2 b^2 c^2 \ell \alpha + b^4 c^2 \alpha^2 + 2 c \ell \alpha r_y + 2 b^2 c \alpha^2 r_y + \alpha^2 r_y^2}} \right\}$$


In[*]:= A3 := ℓ c γ + c Subscript[r, x];
               [下角标]

B3 := 1 - c Subscript[r, x];
               [下角标]

Simplify[val[[2]] - (-A3 / 2 - (B3 β) / 2 + (1 / 2) Sqrt[(A3 + B3 β) ^ 2 - 4 ℓ c β γ])]
[化简] [平方根]

(* Check the form of λ *)
[校验]

Simplify[vec[[2]] - ((1 / (2 (1 - A3) β)) *
               (-A3 + B3 β + Sqrt[(A3 - B3 β) ^ 2 + 4 c Subscript[r, x] β (1 - A3)]), 1]
               [平方根] [下角标]

(* Check the form of corresponding eigenvector. *)
[校验]

)]

Out[*]=
0

Out[*]=
{0, 0}

```